Change HttpResponseLine to HttpResponsePart.
Because this describes what happens in the server more accurately:
requests are processed line by line, but responses are not.

HttpResponse.v
@@ -5,28 +5,28 @@ Require Import Utility.
 
 (** Definitions of HTTP response. **)
 
-Inductive HttpResponseLine : Type :=
-| Res_HeaderLine : string -> HttpResponseLine
-| Res_BodyLine : string -> HttpResponseLine.
+Inductive HttpResponsePart : Type :=
+| Res_HeaderPart : string -> HttpResponsePart
+| Res_BodyPart : string -> HttpResponsePart.
 
-Definition HttpResponse : Type := list HttpResponseLine.
+Definition HttpResponse : Type := list HttpResponsePart.
 
 (** Definitions of what a well formed HTTP response is. *)
 
 Inductive response_body : HttpResponse -> Prop :=
 | rb_cons_nil : forall s,
-    response_body (Res_BodyLine s :: nil)
+    response_body (Res_BodyPart s :: nil)
 | rb_cons_body : forall s res,
     response_body res ->
-    response_body (Res_BodyLine s :: res).
+    response_body (Res_BodyPart s :: res).
 
 Inductive response_header : HttpResponse -> Prop :=
 | rf_cons_body : forall s res,
     response_body res ->
-    response_header (Res_HeaderLine s :: res)
+    response_header (Res_HeaderPart s :: res)
 | rf_cons_header : forall s res,
     response_header res ->
-    response_header (Res_HeaderLine s :: res).
+    response_header (Res_HeaderPart s :: res).
 
 (* A well formed response must be some header lines followed by some body lines.
      That means, header lines can not be between body lines,
@@ -38,7 +38,7 @@ Definition well_formed_response (res: HttpResponse) : Prop := response_header re
 
 Lemma response_body_no_header_line:
   forall res1 res2 s,
-    ~ response_body (res1 ++ Res_HeaderLine s :: res2).
+    ~ response_body (res1 ++ Res_HeaderPart s :: res2).
 Proof.
   intros. induction res1; simpl; intro.
   - inversion H.
@@ -52,12 +52,12 @@ Qed.
 Lemma body_before_header_response_not_well_formed:
   forall res1 res2 s1 s2,
     ~ well_formed_response (res1 ++
-                                 Res_BodyLine s1 :: Res_HeaderLine s2 :: res2).
+                                 Res_BodyPart s1 :: Res_HeaderPart s2 :: res2).
 Proof.
   intros. induction res1; simpl; intro.
   - inversion H.
   - inversion H; subst.
-    + assert (response_body ((res1 ++ Res_BodyLine s1 :: nil) ++ (Res_HeaderLine s2 :: res2))).
+    + assert (response_body ((res1 ++ Res_BodyPart s1 :: nil) ++ (Res_HeaderPart s2 :: res2))).
       { rewrite <- app_assoc. simpl. assumption. }
       eapply response_body_no_header_line. apply H0.
     + unfold well_formed_response in IHres1. contradiction.
